$$
\begin{align}
a&=\frac{s}{\frac{1}{2}t^{2} } \\
\mathrm{d}a&= \frac{\frac{1}{2}t^{2}\mathrm{d}s-st\mathrm{d}t}{\frac{1}{4}t^{4}}
\end{align}
$$

3.1

$$
\begin{align}
u&=\frac{2f(Q_{1}-P_{1})}{N} \\
\mathrm{d}u&=\frac{2f}{N}\mathrm{d}(Q_{1}-P_{1}) \\
&=\frac{4f}{N}\mathrm{d}P
\end{align}
$$

3.2

$$
\begin{align}
\frac{\Delta}{\lambda}&= \frac{ P_{2}-P_{1}+Q_{2}-Q_{1} }{2\lambda} \\
\mathrm{d}\left( \frac{\Delta}{\lambda} \right)&= \frac{2\lambda \cdot 4\mathrm{d}P-2(P_{2}-P_{1}+Q_{2}-Q_{1})\mathrm{d}\lambda}{\lambda^{2}}
 \end{align}
$$

4

$$
\begin{align}
n&= \frac{R-M}{d}+1 \\
\mathrm{d}n&= \frac{d\cdot\mathrm{d}(R-M)-(R-M)\mathrm{d}d}{d^{2}} \\
&=\frac{2d-(R-M)}{d^{2}}\mathrm{d}M
\end{align}
$$
